eve/Src/library/base/mml/sequence.bpl
@@ -95,6 +95,8 @@ axiom (forall<T> a: Seq T, x: T:: {Seq#Occurrences(Seq#Extended(a, x), x)}
   Seq#Occurrences(Seq#Extended(a, x), x) == Seq#Occurrences(a, x) + 1);
 axiom (forall<T> a: Seq T, x: T, y: T :: {Seq#Occurrences(Seq#Extended(a, y), x)}
   x != y ==> Seq#Occurrences(Seq#Extended(a, y), x) == Seq#Occurrences(a, x));
+ // axiom (forall<T> a: Seq T, x: T :: {Seq#Occurrences(a, x)}
+  // !Seq#Has(a, x) ==> Seq#Occurrences(a, x) == 0);
 
 // Are two sequences equal?  
 function Seq#Equal<T>(Seq T, Seq T): bool;
@@ -315,6 +317,9 @@ axiom (forall<T> :: Seq#Drop(Seq#Empty() : Seq T, 0) == Seq#Empty() : Seq T);  /
 
 function Seq#NonNull(s: Seq ref): bool
 { (forall i: int :: { Seq#Item(s, i) } 1 <= i && i <= Seq#Length(s) ==> Seq#Item(s, i) != Void) }
+
+// function Seq#NoDuplicates<T>(s: Seq T): bool
+// { (forall i, j: int :: 1 <= i && i < j && j < Seq#Length(s) ==> Seq#Item(s, i) != Seq#Item(s, j)) }
 
 // Type property
 function {: inline } Seq#ItemsType(heap: HeapType, s: Seq ref, t: Type): bool 
