eve/Src/framework/eiffel2boogie/translation/e2b_routine_translator.e
@@ -693,17 +693,19 @@ feature -- Translation: Functions
 			create l_fcall.make (l_function.name, l_function.type)
 
 				-- Arguments
-			l_function.add_argument ("heap", types.heap)
-			l_function.add_argument ("current", types.ref)
-			l_fcall.add_argument (factory.old_ (factory.global_heap))
-			l_fcall.add_argument (factory.std_current)
-			across
-				arguments_of_current_feature as i
-			loop
-				create l_arg.make (i.item.name, i.item.boogie_type)
-				translation_pool.add_type (i.item.type)
-				l_function.add_argument (i.item.name, i.item.boogie_type)
-				l_fcall.add_argument (l_arg)
+			if not current_feature.is_once then
+				l_function.add_argument ("heap", types.heap)
+				l_function.add_argument ("current", types.ref)
+				l_fcall.add_argument (factory.old_ (factory.global_heap))
+				l_fcall.add_argument (factory.std_current)
+				across
+					arguments_of_current_feature as i
+				loop
+					create l_arg.make (i.item.name, i.item.boogie_type)
+					translation_pool.add_type (i.item.type)
+					l_function.add_argument (i.item.name, i.item.boogie_type)
+					l_fcall.add_argument (l_arg)
+				end
 			end
 
 				-- Definition
@@ -722,7 +724,7 @@ feature -- Translation: Functions
 			create l_translator.make
 			l_translator.set_context (current_feature, current_type)
 			l_reads := read_expressions_of (contracts_of (current_feature, current_type).reads, l_translator).full_objects
-			if not (across l_reads as e some factory.universe.same_expression (e.item) end) then
+			if not current_feature.is_once and not (across l_reads as e some factory.universe.same_expression (e.item) end) then
 				generate_frame_axiom (l_function)
 			end
 		end
@@ -874,9 +876,15 @@ feature -- Translation: Functions
 			across l_function.arguments as a loop
 				l_fcall.add_argument (a.item.entity)
 			end
-			create l_forall.make (factory.implies_ (
-				factory.is_heap (l_translator.entity_mapping.heap),
-				frame_definition (l_exprs, l_fcall)))
+			if a_read and not helper.is_feature_status (a_feature, "inv_unfriendly") then
+				create l_forall.make (factory.implies_ (
+					factory.is_heap (l_translator.entity_mapping.heap),
+					frame_definition (l_exprs, l_fcall, << factory.entity ("closed", types.field (types.bool)), factory.entity ("owner", types.field (types.ref)) >>)))
+			else
+				create l_forall.make (factory.implies_ (
+					factory.is_heap (l_translator.entity_mapping.heap),
+					frame_definition (l_exprs, l_fcall, <<>>)))
+			end
 			across l_function.arguments as a
 			loop
 				l_forall.add_bound_variable (a.item.entity)
@@ -950,23 +958,19 @@ feature {NONE} -- Translation: Functions
 			l_expr_translator: E2B_CONTRACT_EXPRESSION_TRANSLATOR
 			l_axiom: IV_AXIOM
 			l_forall: IV_FORALL
-			l_pre, l_post: IV_EXPRESSION
-			l_pre_call, l_fcall, l_trigger_call: IV_FUNCTION_CALL
+			l_post: IV_EXPRESSION
+			l_fcall, l_pre_call, l_trigger_call: IV_FUNCTION_CALL
 		do
 			create l_fcall.make (a_function.name, a_function.type)
 			create l_pre_call.make (name_translator.boogie_function_precondition (a_function.name), types.bool)
---			create l_free_pre_call.make (name_translator.boogie_free_function_precondition (a_function.name), types.bool)
 			create l_trigger_call.make (name_translator.boogie_function_trigger (a_function.name), types.bool)
 			across a_function.arguments as args loop
 				l_fcall.add_argument (args.item.entity)
 				l_pre_call.add_argument (args.item.entity)
---				l_free_pre_call.add_argument (args.item.entity)
 				l_trigger_call.add_argument (args.item.entity)
 			end
---			l_pre := factory.and_ (l_free_pre_call, l_pre_call)
-			l_pre := l_pre_call
 
-			l_expr_translator := translator_for_function (a_function)
+			l_expr_translator := translator_for_function (l_fcall)
 			if helper.is_functional (current_feature) then
 					-- Generate `l_post' from body					
 				if attached Context.byte_code and then functional_body (Context.byte_code.compound) /= Void then
@@ -987,11 +991,16 @@ feature {NONE} -- Translation: Functions
 						current_feature.type.is_attached))
 			end
 
-			if helper.is_feature_status (current_feature, "opaque") then
-				create l_forall.make (factory.implies_ (factory.and_ (l_pre, l_trigger_call), l_post))
+			if current_feature.is_once then
+				create l_forall.make (l_post)
+				check attached {IV_ENTITY} l_expr_translator.entity_mapping.heap as ent then
+					l_forall.add_bound_variable (ent)
+				end
+			elseif helper.is_feature_status (current_feature, "opaque") then
+				create l_forall.make (factory.implies_ (factory.and_ (l_pre_call, l_trigger_call), l_post))
 				l_forall.add_trigger (l_trigger_call)
 			else
-				create l_forall.make (factory.implies_ (l_pre, l_post))
+				create l_forall.make (factory.implies_ (l_pre_call, l_post))
 				l_forall.add_trigger (l_fcall)
 			end
 			l_forall.bound_variables.append (a_function.arguments)
@@ -1013,22 +1022,14 @@ feature {NONE} -- Translation: Functions
 			end
 		end
 
-	translator_for_function (a_function: IV_FUNCTION): E2B_CONTRACT_EXPRESSION_TRANSLATOR
-			-- Translator that maps `Result' to the invocation of `a_function'.
-		local
-			l_function_call: IV_FUNCTION_CALL
+	translator_for_function (a_fcall: IV_EXPRESSION): E2B_CONTRACT_EXPRESSION_TRANSLATOR
+			-- Translator that maps `Result' to the invocation of `a_fcall'.
 		do
 			create Result.make
 			Result.entity_mapping.set_current (create {IV_ENTITY}.make ("current", types.ref))
 			Result.entity_mapping.set_heap (create {IV_ENTITY}.make ("heap", types.heap))
 			Result.set_context (current_feature, current_type)
-			create l_function_call.make (a_function.name, a_function.type)
-			l_function_call.add_argument (Result.entity_mapping.heap)
-			l_function_call.add_argument (Result.entity_mapping.current_expression)
-			across arguments_of_current_feature as i loop
-				l_function_call.add_argument (create {IV_ENTITY}.make(i.item.name, i.item.boogie_type))
-			end
-			Result.entity_mapping.set_result (l_function_call)
+			Result.entity_mapping.set_result (a_fcall)
 		end
 
 	generate_frame_axiom (a_function: IV_FUNCTION)
