eve/Src/framework/eiffel2boogie/translation/e2b_routine_translator_base.e
@@ -374,7 +374,7 @@ feature -- Helper functions: contracts
 				(a_mods.model_objects.is_empty or else a_mods.model_objects.first.objects.first = Void)
 		end
 
-	frame_definition (a_mods: like modify_expressions_of; a_lhs: IV_EXPRESSION): IV_FORALL
+	frame_definition (a_mods: like modify_expressions_of; a_lhs: IV_EXPRESSION; a_excluded_fields: ARRAY [IV_ENTITY]): IV_FORALL
 			-- Expression that claims that `a_lhs' is the frame encoded in `a_mods'
 			-- (forall o, f :: a_lhs[o, f] <==> is_partially_modifiable[o, f] || is_model_modifiable[o, f] || is_fully_modifiable[o])
 		local
@@ -416,7 +416,13 @@ feature -- Helper functions: contracts
 				l_expr := factory.or_clean (l_expr, factory.and_ (is_object_in_frame (l_o, r.objects), l_f_conjunct))
 			end
 				-- Go over fully modifiable objects
-			l_expr := factory.or_clean (l_expr, is_object_in_frame (l_o, a_mods.full_objects))
+				-- (and exclude `a_excluded_fields')
+			l_f_conjunct := factory.true_
+			across a_excluded_fields as f loop
+				l_f_conjunct := factory.and_clean (l_f_conjunct, factory.not_equal (l_f, f.item))
+			end
+			l_expr := factory.or_clean (l_expr,
+				factory.and_clean (is_object_in_frame (l_o, a_mods.full_objects), l_f_conjunct))
 				-- Finally create the quantifier				
 			create Result.make (factory.equiv (l_access, l_expr))
 			Result.add_type_variable (l_type_var.name)
