eve/Src/library/base/base2/dispenser/v_stack.e
@@ -26,12 +26,12 @@ feature -- Extension
 
 feature -- Specification
 
-	is_model_equal (other: ANY): BOOLEAN
+	is_model_equal (other: like Current): BOOLEAN
 			-- Is the abstract state of `Current' equal to that of `other'?
 		note
 			status: ghost, functional
 		do
-			Result := attached {V_STACK [G]} other as s and then sequence ~ s.sequence
+			Result := sequence ~ other.sequence
 		end
 
 note
